vale/specs/interop/Interop.X64.fsti
@@ -252,13 +252,17 @@ let prediction_pre_rel_t (c:TS.tainted_code) (args:arity_ok arg) =
     h0:mem_roots args ->
     prop
 
+let return_val_t (sn:TS.traceState) = r:UInt64.t{UInt64.v r == BS.eval_reg MS.Rax sn.TS.state}
+let return_val (sn:TS.traceState) : return_val_t sn =
+  UInt64.uint_to_t (BS.eval_reg MS.Rax sn.TS.state)
+
 let prediction_post_rel_t (c:TS.tainted_code) (num_b8_slots:max_slots) (args:arity_ok arg) =
     h0:mem_roots args ->
     s0:TS.traceState ->
     push_h0:mem_roots args ->
     alloc_push_h0:mem_roots args ->
     b:stack_buffer num_b8_slots{mem_roots_p alloc_push_h0 (arg_of_sb b::args)} ->
-    (nat & mem) ->
+    (UInt64.t & nat & mem) ->
     sn:TS.traceState ->
     prop
 
@@ -295,9 +299,9 @@ let prediction_post
     (push_h0:mem_roots args)
     (alloc_push_h0:mem_roots args)
     (sb:stack_buffer num_b8_slots{mem_roots_p alloc_push_h0 (arg_of_sb sb::args)})
-    (fuel_mem:nat & mem) =
+    (rax_fuel_mem:(UInt64.t & nat & mem)) =
   let s_args = arg_of_sb sb :: args in
-  let fuel, final_mem = fuel_mem in
+  let rax, fuel, final_mem = rax_fuel_mem in
   Some? (TS.taint_eval_code c fuel s0) /\ (
     let s1 = Some?.v (TS.taint_eval_code c fuel s0) in
     let h1 = hs_of_mem final_mem in
@@ -306,7 +310,8 @@ let prediction_post
     mem_roots_p h1 s_args /\
     down_mem (mk_mem s_args h1) == s1.TS.state.BS.mem /\
     calling_conventions s0 s1 /\
-    post_rel h0 s0 push_h0 alloc_push_h0 sb fuel_mem s1
+    rax == return_val s1 /\
+    post_rel h0 s0 push_h0 alloc_push_h0 sb rax_fuel_mem s1
   )
 
 let prediction
@@ -321,7 +326,7 @@ let prediction
   push_h0:mem_roots args ->
   alloc_push_h0:mem_roots args ->
   b:stack_buffer num_b8_slots{mem_roots_p h0 args /\ mem_roots_p alloc_push_h0 (arg_of_sb b::args)} ->
-  Ghost (nat & mem)
+  Ghost (UInt64.t & nat & mem)
     (requires prediction_pre down_mem c num_b8_slots args pre_rel h0 s0 push_h0 alloc_push_h0 b)
     (ensures prediction_post down_mem c num_b8_slots args post_rel h0 s0 push_h0 alloc_push_h0 b)
 
@@ -337,7 +342,7 @@ type as_lowstar_sig_ret =
       final_mem:mem ->
       as_lowstar_sig_ret
 
-let als_ret = Ghost.erased as_lowstar_sig_ret
+let als_ret = UInt64.t & Ghost.erased as_lowstar_sig_ret
 
 [@__reduce__]
 let as_lowstar_sig_post
@@ -352,7 +357,8 @@ let as_lowstar_sig_post
     (ret:als_ret)
     (h1:HS.mem) =
   (* write it this way to be reduction friendly *)
-  let ret = Ghost.reveal ret in
+  let rax = fst ret in
+  let ret = Ghost.reveal (snd ret) in
   num_b8_slots == As_lowstar_sig_ret?.num_b8_slots ret /\
   args == As_lowstar_sig_ret?.args ret /\
  (let push_h0 = As_lowstar_sig_ret?.push_h0 ret in
@@ -363,8 +369,8 @@ let as_lowstar_sig_post
   let s0 = fst (create_initial_trusted_state num_b8_slots args down_mem alloc_push_h0 b) in
   let pre_pop = hs_of_mem final_mem in
   prediction_pre down_mem c num_b8_slots args pre_rel h0 s0 push_h0 alloc_push_h0 b /\
-  (fuel, final_mem) == predict h0 s0 push_h0 alloc_push_h0 b /\
-  prediction_post down_mem c num_b8_slots args post_rel h0 s0 push_h0 alloc_push_h0 b (fuel, final_mem) /\
+  (rax, fuel, final_mem) == predict h0 s0 push_h0 alloc_push_h0 b /\
+  prediction_post down_mem c num_b8_slots args post_rel h0 s0 push_h0 alloc_push_h0 b (rax, fuel, final_mem) /\
   FStar.HyperStack.ST.equal_domains alloc_push_h0 pre_pop /\
   HS.poppable pre_pop /\
   h1 == HS.pop pre_pop)
@@ -382,7 +388,7 @@ let as_lowstar_sig_post_weak
     (ret:als_ret)
     (h1:HS.mem) =
   (* write it this way to be reduction friendly *)
-  let ret = Ghost.reveal ret in
+  let ret = Ghost.reveal (snd ret) in
   num_b8_slots == As_lowstar_sig_ret?.num_b8_slots ret /\
   args == As_lowstar_sig_ret?.args ret /\
  (let push_h0 = As_lowstar_sig_ret?.push_h0 ret in
@@ -394,11 +400,11 @@ let as_lowstar_sig_post_weak
   let pre_pop = hs_of_mem final_mem in
   (exists fuel
      final_mem
-     _s1.
+     s1.
      let pre_pop = hs_of_mem final_mem in
      HS.poppable pre_pop /\
      h1 == HS.pop pre_pop /\
-     post_rel h0 s0 push_h0 alloc_push_h0 b (fuel, final_mem) _s1))
+     post_rel h0 s0 push_h0 alloc_push_h0 b (return_val s1, fuel, final_mem) s1))
 
 [@__reduce__]
 let as_lowstar_sig (c:TS.tainted_code) =
